## Derivatives

$$ \frac{f(x + dx) - f(x)}{dx} = \frac{df}{dx} = f\prime(x) $$

$$ \frac{d(f(x) + g(x))}{dx} = \frac{f(x + dx) + g(x + dx) - f(x) -g(x)}{dx} = \frac{f(x + dx) - f(x)}{dx} + \frac{g(x + dx) - g(x)}{dx} = \frac{df}{dx} + \frac{dg}{dx} $$

$$ (f(x) + g(x))\prime = f\prime(x) + g\prime(x) $$

$$ f(x + dx) = f(x) + df $$

$$ \frac{d(f(x)g(x))}{dx} = \frac{(f(x) + df)(g(x) + dg) - f(x)g(x)}{dx} = \frac{f(x)g(x) + f(x)dg + dfg(x) + dfdg - f(x)g(x)}{dx} = f(x)\frac{dg}{dx} + \frac{df}{dx}g(x) + \frac{dfdg}{dx} $$
