## Complex numbers

$$ i = \sqrt{-1} $$

$$ a + bi = c + di \iff c = a, d = b $$

$$ (a + bi)(c + di) = ac + adi + bci + bdii = ac + adi + bci - bd = (ac - bd) + (ad + bc)i $$

$$ (a + bi)^2 = (aa - bb) + (ab + ab)i = (a^2 - b^2) + 2abi $$

### back to calculus

$$ \sum\limits_{n=0}^{\infty}C_n x^n = e^x $$

$$ \sum\limits_{n=0}^{\infty}C_n n x^{n - 1} = e^x = \sum\limits_{n=0}^{\infty}C_n x^n $$

$$ \sum\limits_{n=0}^{\infty}C_n n x^{n - 1} = \sum\limits_{n=-1}^{\infty}C_{n + 1} (n + 1) x^n = c_0 0 x^{-1} + \sum\limits_{n=0}^{\infty}C_{n + 1} (n + 1) x^n = \sum\limits_{n=0}^{\infty}C_n x^n $$

$$ C_{n + 1} (n + 1) = C_n $$

$$ C_{n + 1} = \frac{C_n}{n + 1} $$

$$ C_n = \frac{C_{n - 1}}{n} $$

$$ e^0 = 1 $$

$$ C_0 = 1 $$

$$ C_n = \frac{1}{n!} $$

$$ e^x = \sum\limits_{n=0}^{\infty}\frac{x^n}{n!} $$
